src/ocaml/extraction/Nat0.ml
@@ -5,6 +5,6 @@ let rec add = (+)
 
 (** val sub : int -> int -> int **)
 
-let rec sub = fun n m -> Pervasives.max 0 (n-m)
+let rec sub = fun n m -> Stdlib.max 0 (n-m)
 
 
