src/ocaml/extraction/seq.mli
@@ -2,7 +2,6 @@ open Bool
 open Datatypes
 open Eqtype
 open Ssrbool
-open Ssreflect
 open Ssrnat
 
 val size : 'a1 list -> int
