src/HiFirrtl.v
@@ -37,16 +37,179 @@ Section HiFirrtl.
   .
 
   (** equality of hfexpr and href are decidable *)
-  Axiom hfexpr_eq_dec : forall {x y : hfexpr}, {x = y} + {x <> y}.
-  Parameter hfexpr_eqn : forall (x y : hfexpr), bool.
-  Axiom hfexpr_eqP : Equality.axiom hfexpr_eqn.
+  Lemma hfexpr_eq_dec : forall {x y : hfexpr}, {x = y} + {x <> y}
+  with href_eq_dec : forall {x y : href}, {x = y} + {x <> y}.
+  (** clear hfexpr_eq_dec.
+    destruct x, y ; decide equality ; try (apply fgtyp_eq_dec) ; try (apply ucast_eq_dec) ;
+    try (apply eunop_eq_dec) ; try (apply ebinop_eq_dec).
+    + destruct (b1 == b2) eqn: H ; move /eqP : H => H ;
+      first (by left  ; exact H) ;
+      last  (by right ; exact H).
+    1-7, 14, 21, 28, 35, 42: destruct (b0 == b1) eqn: H ; move /eqP : H => H ;
+      first (by left  ; exact H) ;
+      last  (by right ; exact H).
+    1-36: destruct (b == b0) eqn: H ; move /eqP : H => H ;
+      first (by left  ; exact H) ;
+      last  (by right ; exact H).
+  * clear href_eq_dec.
+    destruct x, y ; decide equality ; try apply Nat.eq_dec.
+    + destruct (s1 == s2) eqn: H ; move /eqP : H => H ;
+      first (by left  ; exact H) ;
+      last  (by right ; exact H).
+    1,5,7,17,21,23,25,29,31: destruct (v == v0) eqn: H ; move /eqP : H => H ;
+      first (by left  ; exact H) ;
+      last  (by right ; exact H).
+    1,3-5,13,18: destruct (s0 == s1) eqn: H ; move /eqP : H => H ;
+      first (by left  ; exact H) ;
+      last  (by right ; exact H).
+    1,2,6,8,10,14: destruct (v0 == v1) eqn: H ; move /eqP : H => H ;
+      first (by left  ; exact H) ;
+      last  (by right ; exact H).
+    1,3-10: destruct (s == s0) eqn: H ; move /eqP : H => H ;
+      first (by left  ; exact H) ;
+      last  (by right ; exact H).
+    + destruct (v1 == v2) eqn: H ; move /eqP : H => H ;
+      first (by left  ; exact H) ;
+      last  (by right ; exact H).
+  Qed.*) Admitted.
+  Fixpoint hfexpr_eqn (x y : hfexpr) : bool :=
+  match x, y with
+  | Econst tx bx, Econst ty by_ => (tx == ty) && (bx == by_)
+  | Ecast ux ex, Ecast uy ey => (ux == uy) && hfexpr_eqn ex ey
+  | Eprim_unop ux ex, Eprim_unop uy ey => (ux == uy) && hfexpr_eqn ex ey
+  | Eprim_binop bx ex fx, Eprim_binop by_ ey fy => (bx == by_) && hfexpr_eqn ex ey && hfexpr_eqn fx fy
+  | Emux ex fx gx, Emux ey fy gy => hfexpr_eqn ex ey && hfexpr_eqn fx fy && hfexpr_eqn gx gy
+  | Eref rx, Eref ry => href_eqn rx ry
+  | _, _ => false
+  end
+  with href_eqn (x y : href) : bool :=
+  match x, y with
+  | Eid vx, Eid vy => vx == vy
+  | Esubfield rx vx, Esubfield ry vy => href_eqn rx ry && (vx == vy)
+  | Esubindex rx nx, Esubindex ry ny => href_eqn rx ry && (nx == ny)
+  | Esubaccess rx ex, Esubaccess ry ey => href_eqn rx ry && hfexpr_eqn ex ey
+  | _, _ => false
+  end.
+  Lemma hfexpr_eqP : (*Equality.axiom hfexpr_eqn*)
+        forall x y : hfexpr, reflect (x = y) (hfexpr_eqn x y)
+  with href_eqP : (*Equality.axiom href_eqn*)
+        forall x y : href, reflect (x = y) (href_eqn x y).
+  Proof.
+  (** clear hfexpr_eqP.
+    induction x, y ; simpl ;
+          try (apply ReflectF ; discriminate).
+    + destruct (f == f0) eqn: Hf ; move /eqP : Hf => Hf ;
+            last by (apply ReflectF ; injection ; done).
+      rewrite Hf andTb.
+      destruct (b == b0) eqn: Hb ; move /eqP : Hb => Hb ;
+            last by (apply ReflectF ; injection ; done).
+      rewrite Hb.
+      apply ReflectT ; reflexivity.
+    + destruct (u == u0) eqn: Hu ; move /eqP : Hu => Hu ;
+            last by (apply ReflectF ; injection ; done).
+      rewrite Hu andTb.
+      specialize (IHx y) ; apply reflect_iff in IHx.
+      destruct (hfexpr_eqn x y) ;
+            last by (apply ReflectF ; injection ; intro ;
+                     destruct IHx as [IHx _] ; apply IHx in H0 ; done).
+      destruct IHx as [_ IHx] ; rewrite IHx //.
+      apply ReflectT ; reflexivity.
+    + destruct (e == e0) eqn: He ; move /eqP : He => He ;
+            last by (apply ReflectF ; injection ; done).
+      rewrite He andTb.
+      specialize (IHx y) ; apply reflect_iff in IHx.
+      destruct (hfexpr_eqn x y) ;
+            last by (apply ReflectF ; injection ; intro ;
+                     destruct IHx as [IHx _] ; apply IHx in H0 ; done).
+      destruct IHx as [_ IHx] ; rewrite IHx //.
+      apply ReflectT ; reflexivity.
+    + destruct (e == e0) eqn: He ; move /eqP : He => He ;
+            last by (apply ReflectF ; injection ; done).
+      rewrite He andTb.
+      specialize (IHx1 y1) ; apply reflect_iff in IHx1.
+      destruct (hfexpr_eqn x1 y1) ;
+            last by (apply ReflectF ; injection ; intros _ H0 ;
+                     destruct IHx1 as [IHx1 _] ; apply IHx1 in H0 ; done).
+      destruct IHx1 as [_ IHx1] ; rewrite IHx1 //.
+      specialize (IHx2 y2) ; apply reflect_iff in IHx2.
+      destruct (hfexpr_eqn x2 y2) ;
+            last by (apply ReflectF ; injection ; intros H0 ;
+                     destruct IHx2 as [IHx2 _] ; apply IHx2 in H0 ; done).
+      destruct IHx2 as [_ IHx2] ; rewrite IHx2 //.
+      apply ReflectT ; reflexivity.
+    + specialize (IHx1 y1) ; apply reflect_iff in IHx1.
+      destruct (hfexpr_eqn x1 y1) ;
+            last by (apply ReflectF ; injection ; intros _ _ H0 ;
+                     destruct IHx1 as [IHx1 _] ; apply IHx1 in H0 ; done).
+      destruct IHx1 as [_ IHx1] ; rewrite IHx1 //.
+      specialize (IHx2 y2) ; apply reflect_iff in IHx2.
+      destruct (hfexpr_eqn x2 y2) ;
+            last by (apply ReflectF ; injection ; intros _ H0 ;
+                     destruct IHx2 as [IHx2 _] ; apply IHx2 in H0 ; done).
+      destruct IHx2 as [_ IHx2] ; rewrite IHx2 //.
+      specialize (IHx3 y3) ; apply reflect_iff in IHx3.
+      destruct (hfexpr_eqn x3 y3) ;
+            last by (apply ReflectF ; injection ; intros H0 ;
+                     destruct IHx3 as [IHx3 _] ; apply IHx3 in H0 ; done).
+      destruct IHx3 as [_ IHx3] ; rewrite IHx3 //.
+      apply ReflectT ; reflexivity.
+    + specialize (IHx1 y1) ; apply reflect_iff in IHx1.
+      destruct (hfexpr_eqn x1 y1) ;
+            last by (apply ReflectF ; injection ; intros _ H0 ;
+                     destruct IHx1 as [IHx1 _] ; apply IHx1 in H0 ; done).
+      destruct IHx1 as [_ IHx1] ; rewrite IHx1 //.
+      specialize (IHx2 y2) ; apply reflect_iff in IHx2.
+      destruct (hfexpr_eqn x2 y2) ;
+            last by (apply ReflectF ; injection ; intros H0 ;
+                     destruct IHx2 as [IHx2 _] ; apply IHx2 in H0 ; done).
+      destruct IHx2 as [_ IHx2] ; rewrite IHx2 //.
+      apply ReflectT ; reflexivity.
+    + specialize (href_eqP h h0) ; apply reflect_iff in href_eqP.
+      destruct (href_eqn h h0) ;
+            last by (apply ReflectF ; injection ; intros H0 ;
+                     destruct href_eqP as [href_eqP _] ; apply href_eqP in H0 ; done).
+      destruct href_eqP as [_ href_eqP] ; rewrite href_eqP //.
+      apply ReflectT ; reflexivity.
+  * clear href_eqP.
+    induction x, y ; simpl ;
+          try (apply ReflectF ; discriminate).
+    + destruct (s == s0) eqn: Hs ; move /eqP : Hs => Hs ;
+            last by (apply ReflectF ; injection ; done).
+      rewrite Hs.
+      apply ReflectT ; reflexivity.
+    + specialize (IHx y) ; apply reflect_iff in IHx.
+      destruct (href_eqn x y) ;
+            last by (apply ReflectF ; injection ; intros _ H0 ;
+                     destruct IHx as [IHx _] ; apply IHx in H0 ; done).
+      destruct IHx as [_ IHx] ; rewrite IHx //.
+      destruct (v == v0) eqn: Hv ; move /eqP : Hv => Hv ;
+            last by (apply ReflectF ; injection ; done).
+      rewrite Hv.
+      apply ReflectT ; reflexivity.
+    + specialize (IHx y) ; apply reflect_iff in IHx.
+      destruct (href_eqn x y) ;
+            last by (apply ReflectF ; injection ; intros _ H0 ;
+                     destruct IHx as [IHx _] ; apply IHx in H0 ; done).
+      destruct IHx as [_ IHx] ; rewrite IHx //.
+      destruct (n == n0) eqn: Hn ; move /eqP : Hn => Hn ;
+            last by (apply ReflectF ; injection ; done).
+      rewrite Hn.
+      apply ReflectT ; reflexivity.
+    + specialize (IHx y) ; apply reflect_iff in IHx.
+      destruct (href_eqn x y) ;
+            last by (apply ReflectF ; injection ; intros _ H0 ;
+                     destruct IHx as [IHx _] ; apply IHx in H0 ; done).
+      destruct IHx as [_ IHx] ; rewrite IHx //.
+      specialize (hfexpr_eqP h h0) ; apply reflect_iff in hfexpr_eqP.
+      destruct (hfexpr_eqn h h0) ;
+            last by (apply ReflectF ; injection ; intros H0 ;
+                     destruct hfexpr_eqP as [hfexpr_eqP _] ; apply hfexpr_eqP in H0 ; done).
+      destruct hfexpr_eqP as [_ hfexpr_eqP] ; rewrite hfexpr_eqP //.
+      apply ReflectT ; reflexivity.
+  Qed.*) Admitted.
   Canonical hfexpr_eqMixin := EqMixin hfexpr_eqP.
-  Canonical hfexpr_eqType := Eval hnf in EqType hfexpr hfexpr_eqMixin.
-
-  Axiom href_eq_dec : forall {x y : href}, {x = y} + {x <> y}.
-  Parameter href_eqn : forall (x y : href), bool.
-  Axiom href_eqP : Equality.axiom href_eqn.
   Canonical href_eqMixin := EqMixin href_eqP.
+  Canonical hfexpr_eqType := Eval hnf in EqType hfexpr hfexpr_eqMixin.
   Canonical href_eqType := Eval hnf in EqType href href_eqMixin.
 
   (****** Statements ******)
@@ -79,9 +242,71 @@ Section HiFirrtl.
         read_write : ruw
       }.
 
+  Lemma hfmem_eq_dec : forall {x y : hfmem}, {x = y} + {x <> y}.
+  Proof.  decide equality ; try decide equality ;
+          try apply mem_port_eq_dec ;
+          try apply fgtyp_eq_dec ; try apply Nat.eq_dec ; try apply ffield_eq_dec.
+  Qed.
+  Definition hfmem_eqn (x y : hfmem) : bool :=
+  (data_type x == data_type y) && (depth x == depth y) &&
+  (reader x == reader y) && (writer x == writer y) &&
+  (read_latency x == read_latency y) && (write_latency x == write_latency y) &&
+  (read_write x == read_write y).
+  Lemma hfmem_eqP : Equality.axiom hfmem_eqn.
+  Proof.
+  unfold Equality.axiom, hfmem_eqn.
+  destruct x, y ; simpl.
+  destruct (data_type0 == data_type1) eqn: Hdt ; move /eqP : Hdt => Hdt ;
+        last by (apply ReflectF ; contradict Hdt ; injection Hdt ; done).
+  rewrite Hdt andTb.
+  destruct (depth0 == depth1) eqn: Hdp ; move /eqP : Hdp => Hdp ;
+        last by (apply ReflectF ; contradict Hdp ; injection Hdp ; done).
+  rewrite Hdp andTb.
+  destruct (reader0 == reader1) eqn: Hrd ; move /eqP : Hrd => Hrd ;
+        last by (apply ReflectF ; contradict Hrd ; injection Hrd ; done).
+  rewrite Hrd andTb.
+  destruct (writer0 == writer1) eqn: Hwr ; move /eqP : Hwr => Hwr ;
+        last by (apply ReflectF ; contradict Hwr ; injection Hwr ; done).
+  rewrite Hwr andTb.
+  destruct (read_latency0 == read_latency1) eqn: Hrl ; move /eqP : Hrl => Hrl ;
+        last by (apply ReflectF ; contradict Hrl ; injection Hrl ; done).
+  rewrite Hrl andTb.
+  destruct (write_latency0 == write_latency1) eqn: Hwl ; move /eqP : Hwl => Hwl ;
+        last by (apply ReflectF ; contradict Hwl ; injection Hwl ; done).
+  rewrite Hwl andTb.
+  destruct (read_write0 == read_write1) eqn: Hrw ; move /eqP : Hrw => Hrw ;
+        last by (apply ReflectF ; contradict Hrw ; injection Hrw ; done).
+  rewrite Hrw.
+  apply ReflectT ; reflexivity.
+  Qed.
+  Canonical hfmem_eqMixin := EqMixin hfmem_eqP.
+  Canonical hfmem_eqType := Eval hnf in EqType hfmem hfmem_eqMixin.
+
   Inductive rst : Type :=
   | NRst : rst
-  | Rst : hfexpr -> hfexpr -> rst.
+  | Rst : hfexpr (* reset trigger signal *) -> hfexpr (* reset value *) -> rst.
+
+  Lemma rst_eq_dec : forall {x y : rst}, {x = y} + {x <> y}.
+  Proof.  decide equality ; apply hfexpr_eq_dec.  Qed.
+  Definition rst_eqn (x y : rst) : bool :=
+  match x, y with
+  | NRst, NRst => true
+  | Rst t1 r1, Rst t2 r2 => (t1 == t2) && (r1 == r2)
+  | _, _ => false
+  end.
+  Lemma rst_eqP : Equality.axiom rst_eqn.
+  Proof.
+  unfold Equality.axiom, rst_eqn ; intros.
+  destruct x, y ; try (apply ReflectF ; discriminate) ; try (apply ReflectT ; reflexivity).
+  destruct (h == h1) eqn: H1 ; move /eqP : H1 => H1.
+  * rewrite andTb ; destruct (h0 == h2) eqn: H2 ; move /eqP : H2 => H2.
+    + apply ReflectT ; rewrite H1 H2 ; reflexivity.
+    + apply ReflectF ; contradict H2 ; injection H2 ; done.
+  * rewrite andFb ; apply ReflectF.
+    contradict H1 ; injection H1 ; done.
+  Qed.
+  Canonical rst_eqMixin := EqMixin rst_eqP.
+  Canonical rst_eqType := Eval hnf in EqType rst rst_eqMixin.
 
   Record hfreg : Type :=
     mk_freg
@@ -91,6 +316,28 @@ Section HiFirrtl.
         clock : hfexpr;
         reset : rst
       }.
+
+  Lemma hfreg_eq_dec : forall {x y : hfreg}, {x = y} + {x <> y}.
+  Proof.  decide equality.  apply rst_eq_dec.  apply hfexpr_eq_dec.  apply ftype_eq_dec.  Qed.
+  Definition hfreg_eqn (x y : hfreg) : bool :=
+  (type x == type y) && (clock x == clock y) && (reset x == reset y).
+  Lemma hfreg_eqP : Equality.axiom hfreg_eqn.
+  Proof.
+  unfold Equality.axiom, hfreg_eqn.
+  destruct x, y ; simpl.
+  destruct (type0 == type1) eqn: Ht ; move /eqP : Ht => Ht ;
+        last by (apply ReflectF ; contradict Ht ; injection Ht ; done).
+  rewrite Ht andTb.
+  destruct (clock0 == clock1) eqn: Hc ; move /eqP : Hc => Hc ;
+        last by (apply ReflectF ; contradict Hc ; injection Hc ; done).
+  rewrite Hc andTb.
+  destruct (reset0 == reset1) eqn: Hr ; move /eqP : Hr => Hr ;
+        last by (apply ReflectF ; contradict Hr ; injection Hr ; done).
+  rewrite Hr.
+  apply ReflectT ; reflexivity.
+  Qed.
+  Canonical hfreg_eqMixin := EqMixin hfreg_eqP.
+  Canonical hfreg_eqType := Eval hnf in EqType hfreg hfreg_eqMixin.
 
   Definition inst_ports : Type := seq var.
 
@@ -119,12 +366,147 @@ Section HiFirrtl.
    Scheme hfstmt_seq_hfstmt_ind := Induction for hfstmt_seq Sort Prop
    with hfstmt_hfstmt_seq_ind := Induction for hfstmt Sort Prop.
 
-   (** equality of hstmt are decidable *)
-  Axiom hfstmt_eq_dec : forall {x y : hfstmt}, {x = y} + {x <> y}.
-  Parameter hfstmt_eqn : forall (x y : hfstmt), bool.
-  Axiom hfstmt_eqP : Equality.axiom hfstmt_eqn.
+   (** equality of hfstmt and hfstmt_seq are decidable *)
+  Lemma hfstmt_eq_dec : forall {x y : hfstmt}, {x = y} + {x <> y}
+  with hfstmt_seq_eq_dec : forall {x y : hfstmt_seq}, {x = y} + {x <> y}.
+  Proof.
+  * clear hfstmt_eq_dec.
+    decide equality ; try (apply ftype_eq_dec) ; try (apply hfreg_eq_dec) ;
+    try (apply hfmem_eq_dec) ; try (apply hfexpr_eq_dec) ; try (apply href_eq_dec).
+    1,2,3,6: destruct (s == s0) eqn: Hss0 ; move /eqP : Hss0 => Hss0 ;
+         first (by left  ; exact Hss0) ;
+         last  (by right ; exact Hss0).
+    destruct (s0 == s2) eqn: Hss0 ; move /eqP : Hss0 => Hss0 ;
+         first (by left  ; exact Hss0) ;
+         last  (by right ; exact Hss0).
+    destruct (s == s1) eqn: Hss0 ; move /eqP : Hss0 => Hss0 ;
+         first (by left  ; exact Hss0) ;
+         last  (by right ; exact Hss0).
+  * clear hfstmt_seq_eq_dec.
+    decide equality.
+  Qed.
+  Fixpoint hfstmt_eqn (x y : hfstmt) : bool :=
+  match x, y with
+  | Sskip, Sskip => true
+  | Swire vx tx, Swire vy ty => (vx == vy) && (tx == ty)
+  | Sreg vx rx, Sreg vy ry => (vx == vy) && (rx == ry)
+  | Smem vx mx, Smem vy my => (vx == vy) && (mx == my)
+  | Sinst vx wx, Sinst vy wy => (vx == vy) && (wx == wy)
+  | Snode vx ex, Snode vy ey => (vx == vy) && (ex == ey)
+  | Sfcnct rx ex, Sfcnct ry ey => (rx == ry) && (ex == ey)
+  (* | Spcnct : href -> hfexpr -> hfstmt *)
+  | Sinvalid rx, Sinvalid ry => rx == ry
+  (* | Sattach : seq var -> fstmt *)
+  | Swhen ex tx fx, Swhen ey ty fy => (ex == ey) && hfstmt_seq_eqn tx ty && hfstmt_seq_eqn fx fy
+  (* | Sstop : hfexpr -> hfexpr -> nat -> hfstmt *)
+  (* | Sprintf (* TBD *) *)
+  (* | Sassert (* TBD *) *)
+  (* | Sassume (* TBD *) *)
+  (* | Sdefname : var -> fstmt *) (* TBD *)
+  (* | Sparam : var -> fexpr -> fstmt *) (* TBD *)
+  | _, _ => false
+  end
+  with hfstmt_seq_eqn (x y : hfstmt_seq) : bool :=
+  match x, y with
+  | Qnil, Qnil => true
+  | Qcons sx qx, Qcons sy qy => hfstmt_eqn sx sy && hfstmt_seq_eqn qx qy
+  | _, _ => false
+  end.
+  Lemma hfstmt_eqP : (*Equality.axiom hfstmt_eqn*)
+              forall x y : hfstmt, reflect (x = y) (hfstmt_eqn x y)
+  with hfstmt_seq_eqP : (*Equality.axiom hfstmt_seq_eqn*)
+              forall x y : hfstmt_seq, reflect (x = y) (hfstmt_seq_eqn x y).
+  Proof.
+  * clear hfstmt_eqP.
+    induction x, y ; simpl ; try (apply ReflectF ; discriminate).
+    + apply ReflectT ; reflexivity.
+    1-3,5: destruct (s == s0) eqn: Hs ; move /eqP : Hs => Hs ;
+               last (by apply ReflectF ; injection ; done) ;
+         rewrite Hs andTb.
+    + destruct (f == f0) eqn: Hf ; move /eqP : Hf => Hf ;
+            last by (apply ReflectF ; injection ; done).
+      rewrite Hf.
+      apply ReflectT ; reflexivity.
+    1-3,6: destruct (h == h0) eqn: Hh ; move /eqP : Hh => Hh ;
+               last (by apply ReflectF ; injection ; done) ;
+         rewrite Hh ;
+         apply ReflectT ; reflexivity.
+    + destruct (s == s1) eqn: Hs ; move /eqP : Hs => Hs ;
+               last (by apply ReflectF ; injection ; done) ;
+            rewrite Hs andTb.
+      destruct (s0 == s2) eqn: Hs0 ; move /eqP : Hs0 => Hs0 ;
+               last (by apply ReflectF ; injection ; done) ;
+            rewrite Hs0.
+      apply ReflectT ; reflexivity.
+    + destruct (h == h1) eqn: Hh ; move /eqP : Hh => Hh ;
+               last (by apply ReflectF ; injection ; done) ;
+            rewrite Hh andTb.
+      destruct (h0 == h2) eqn: Hh0 ; move /eqP : Hh0 => Hh0 ;
+               last (by apply ReflectF ; injection ; done) ;
+            rewrite Hh0.
+      apply ReflectT ; reflexivity.
+    + destruct (h == h2) eqn: Hh ; move /eqP : Hh => Hh ;
+               last (by apply ReflectF ; injection ; done) ;
+            rewrite Hh andTb.
+      generalize (hfstmt_seq_eqP h0 h3) ; intro.
+      apply reflect_iff in H.
+      destruct (hfstmt_seq_eqn h0 h3) ;
+            last by (apply ReflectF ; injection ; intros _ H1 ;
+                     apply H in H1 ; done).
+      destruct H as [_ H] ; rewrite H // andTb.
+      specialize (hfstmt_seq_eqP h1 h4).
+      apply reflect_iff in hfstmt_seq_eqP.
+      destruct (hfstmt_seq_eqn h1 h4) ;
+            last by (apply ReflectF ; injection ; intros H1 ;
+                     apply hfstmt_seq_eqP in H1 ; done).
+      destruct hfstmt_seq_eqP as [_ hfstmt_seq_eqP] ; rewrite hfstmt_seq_eqP //.
+      apply ReflectT ; reflexivity.
+  * clear hfstmt_seq_eqP.
+    induction x, y ; simpl ; try (apply ReflectF ; discriminate).
+    + apply ReflectT ; reflexivity.
+    + specialize (hfstmt_eqP h h0) ; apply reflect_iff in hfstmt_eqP.
+      destruct (hfstmt_eqn h h0) ;
+            last by (apply ReflectF ; injection ; intros _ H0 ;
+                     apply hfstmt_eqP in H0 ; done).
+      destruct hfstmt_eqP as [_ hfstmt_eqP] ; rewrite hfstmt_eqP //.
+      specialize (IHx y) ; apply reflect_iff in IHx.
+      destruct (hfstmt_seq_eqn x y) ;
+            last by (apply ReflectF ; injection ; intros H0 ;
+                     apply IHx in H0 ; done).
+      destruct IHx as [_ IHx] ; rewrite IHx //.
+      apply ReflectT ; reflexivity.
+  Qed.
   Canonical hfstmt_eqMixin := EqMixin hfstmt_eqP.
+  Canonical hfstmt_seq_eqMixin := EqMixin hfstmt_seq_eqP.
   Canonical hfstmt_eqType := Eval hnf in EqType hfstmt hfstmt_eqMixin.
+  Canonical hfstmt_seq_eqType := Eval hnf in EqType hfstmt_seq hfstmt_seq_eqMixin.
+
+   (** hfstmt_seq is an equivalence relation *)
+
+Lemma hfstmt_eqn_refl (x : hfstmt) : x == x
+with hfstmt_seq_eqn_refl (fx : hfstmt_seq) : fx == fx.
+Proof.  all: rewrite eq_refl //.  Qed.
+
+(*Lemma hfstmt_eqn_eq (x y : hfstmt) : x == y <-> x = y
+with hfstmt_seq_eqn_eq (fx fy : hfstmt_seq) : fx == fy <-> fx = fy.
+Proof.
+Admitted.*)
+
+Lemma hfstmt_eqn_sym (x y : hfstmt) : x == y -> y == x
+with hfstmt_seq_eqn_sym (fx fy : hfstmt_seq) : fx == fy -> fy == fx.
+Proof.  all: intro ; rewrite eq_sym //.  Qed.
+
+Lemma hfstmt_eqn_trans (x y z : hfstmt) : x == y -> y == z -> x == z
+with hfstmt_seq_eqn_trans (x y z : hfstmt_seq) : x == y -> y == z -> x == z.
+Proof.  all: intro ; move /eqP : H => H ; rewrite H ; done.  Qed.
+
+Instance hfstmt_seq_eqn_Reflexive : Reflexive (@hfstmt_seq_eqn) := @hfstmt_seq_eqn_refl.
+Instance hfstmt_seq_eqn_Symmetric : Symmetric (@hfstmt_seq_eqn) := @hfstmt_seq_eqn_sym.
+Instance hfstmt_seq_eqn_Transitive : Transitive (@hfstmt_seq_eqn) := @hfstmt_seq_eqn_trans.
+Instance hfstmt_seq_eqn_Equivalence : Equivalence (@hfstmt_seq_eqn) :=
+    { Equivalence_Reflexive := hfstmt_seq_eqn_Reflexive;
+      Equivalence_Symmetric := hfstmt_seq_eqn_Symmetric;
+      Equivalence_Transitive := hfstmt_seq_eqn_Transitive }.
 
    Definition Qhead (default : hfstmt) (s : hfstmt_seq) : hfstmt :=
    match s with Qnil => default
@@ -134,16 +516,197 @@ Section HiFirrtl.
    match s1 with Qnil => s2
                | Qcons h1 tl1 => Qcons h1 (Qcat tl1 s2) end.
 
+   Lemma Qcats0 : forall (ss : hfstmt_seq),
+      Qcat ss Qnil = ss.
+   Proof.
+   induction ss.
+   * by unfold Qcat ; reflexivity.
+   * by simpl Qcat ; rewrite IHss ; reflexivity.
+   Qed.
+
+   Lemma Qcat_nil : forall (ss1 ss2 : hfstmt_seq),
+       Qcat ss1 ss2 = Qnil -> ss1 = Qnil /\ ss2 = Qnil.
+   Proof.
+   induction ss1.
+   * induction ss2 ; first by intros ; split ; reflexivity.
+     simpl Qcat ; discriminate.
+   * intro ; simpl Qcat ; discriminate.
+   Qed.
+
+   Lemma Qcat_assoc : forall (ss1 ss2 ss3 : hfstmt_seq),
+      Qcat (Qcat ss1 ss2) ss3 = Qcat ss1 (Qcat ss2 ss3).
+   Proof.
+   induction ss1.
+   * simpl Qcat ; by reflexivity.
+   * intros ; simpl Qcat ; rewrite IHss1 ; reflexivity.
+   Qed.
+
    Fixpoint Qcatrev (s1 s2 : hfstmt_seq) : hfstmt_seq := (* calculates the reversal of s1, followed by s2 *)
    match s1 with Qnil => s2
                | Qcons h1 tl1 => Qcatrev tl1 (Qcons h1 s2) end.
 
    Definition Qrev (s : hfstmt_seq) : hfstmt_seq := Qcatrev s Qnil.
 
-   Fixpoint Qin (s : hfstmt) (ss : hfstmt_seq) :=
+   Fixpoint Qin (s : hfstmt) (ss : hfstmt_seq) : bool :=
     match ss with Qnil => false
                 | Qcons h tl => (hfstmt_eqn h s) || (Qin s tl)
     end.
+
+  Fixpoint Qremove (s : hfstmt) (ss : hfstmt_seq) : hfstmt_seq :=
+      match ss with
+      | Qnil => Qnil
+      | Qcons h tl =>
+          if hfstmt_eqn h s
+          then tl
+          else Qcons h (Qremove s tl)
+      end.
+
+   Fixpoint Qrcons (ss : hfstmt_seq) (s : hfstmt) : hfstmt_seq :=
+   match ss with
+   | Qnil => Qcons s Qnil
+   | Qcons h tl => Qcons h (Qrcons tl s)
+   end.
+
+   Lemma Qcat_rcons : forall (ss1 : hfstmt_seq) (s : hfstmt) (ss2 : hfstmt_seq),
+      Qcat (Qrcons ss1 s) ss2 = Qcat ss1 (Qcons s ss2).
+   Proof.
+   induction ss1.
+   * unfold Qrcons ; simpl Qcat ; reflexivity.
+   * simpl Qrcons ; simpl Qcat.
+     intros.
+     rewrite IHss1 ; reflexivity.
+   Qed.
+
+   Lemma Qcats1 : forall (ss : hfstmt_seq) (s : hfstmt),
+       Qcat ss (Qcons s Qnil) = Qrcons ss s.
+   Proof.
+   induction ss.
+   * simpl ; reflexivity.
+   * simpl.
+     intro ; rewrite -IHss //.
+   Qed.
+
+Fixpoint Qcatrev_rec (ss1 ss2 : hfstmt_seq) : hfstmt_seq :=
+(* calculates the recursive reversal of ss1, followed by ss2 *)
+  match ss1 with
+    Qnil => ss2
+  | Qcons h1 tl1 =>
+      Qcatrev_rec tl1 (Qcons (Qrev_rec h1) ss2) end
+with Qrev_rec (s : hfstmt) : hfstmt :=
+       match s with
+         Swhen c sst ssf =>
+           Swhen c (Qcatrev_rec sst Qnil) (Qcatrev_rec ssf Qnil)
+       | s => s end.
+   
+Lemma qcatrev_rec0s s : Qcatrev_rec Qnil s = s.
+Proof. by []. Qed.
+
+Lemma qcat0s s : Qcat Qnil s = s.
+Proof. by []. Qed.
+
+Lemma qcats0 s : Qcat s Qnil = s.
+Proof.
+  elim : s => // h h0 /= ->//. 
+Qed.
+
+Variable n0 : nat.  (* numerical parameter for take, drop et al *)
+Variable T : Type.  (* must come before the implicit Type     *)
+Variable x0 : T.    (* default for head/nth *)
+
+Implicit Types x y z : T.
+Implicit Types m n : nat.
+Implicit Type s : seq T.
+Lemma last_ind P :
+  P [::] -> (forall s x, P s -> P (rcons s x)) -> forall s, P s.
+Proof.
+move=> Hnil Hlast s. rewrite -(cat0s s).
+elim : s nil Hnil => [|x s2 IHs] s1 Hs1.
+by rewrite cats0.
+by rewrite -cat_rcons; apply/IHs /Hlast.
+Qed.
+
+Lemma Qrcons_ind' :
+   forall (P : hfstmt_seq -> Prop) (P0 : hfstmt -> Prop),
+       P Qnil ->
+       (forall h : hfstmt, P0 h -> forall h0 : hfstmt_seq, P h0 -> P (Qrcons h0 h)) ->
+       P0 Sskip ->
+       (forall (s : var) (f2 : ftype), P0 (Swire s f2)) ->
+       (forall (s : var) (h : hfreg), P0 (Sreg s h)) ->
+       (forall (s : var) (h : hfmem), P0 (Smem s h)) ->
+       (forall s s0 : var, P0 (Sinst s s0)) ->
+       (forall (s : var) (h : hfexpr), P0 (Snode s h)) ->
+       (forall (h : href) (h0 : hfexpr), P0 (Sfcnct h h0)) ->
+       (forall h : href, P0 (Sinvalid h)) ->
+       (forall (h : hfexpr) (h0 : hfstmt_seq),
+        P h0 -> forall h1 : hfstmt_seq, P h1 -> P0 (Swhen h h0 h1)) ->
+       forall h : hfstmt, P0 h
+
+with Qrcons_seq_ind' :
+forall (P : hfstmt_seq -> Prop) (P0 : hfstmt -> Prop),
+       P Qnil ->
+       (forall h : hfstmt, P0 h -> forall h0 : hfstmt_seq, P h0 -> P (Qrcons h0 h)) ->
+       P0 Sskip ->
+       (forall (s : var) (f2 : ftype), P0 (Swire s f2)) ->
+       (forall (s : var) (h : hfreg), P0 (Sreg s h)) ->
+       (forall (s : var) (h : hfmem), P0 (Smem s h)) ->
+       (forall s s0 : var, P0 (Sinst s s0)) ->
+       (forall (s : var) (h : hfexpr), P0 (Snode s h)) ->
+       (forall (h : href) (h0 : hfexpr), P0 (Sfcnct h h0)) ->
+       (forall h : href, P0 (Sinvalid h)) ->
+       (forall (h : hfexpr) (h0 : hfstmt_seq),
+        P h0 -> forall h1 : hfstmt_seq, P h1 -> P0 (Swhen h h0 h1)) ->
+       forall h : hfstmt_seq, P h.
+Proof.
+  intros. move : h.
+  elim; try done. 
+  intros. apply H9;
+    by apply (Qrcons_seq_ind' P P0).
+
+  intros. rewrite-(qcat0s h). generalize H. move => Hnil.
+  elim : h Qnil H => [|x s2 IHs] s1 Hs1.
+  by rewrite qcats0.
+  rewrite -Qcat_rcons. apply IHs. apply H0; last done.
+  apply (Qrcons_ind' P); try done. 
+Qed.
+  
+Lemma Qrcons_ind :
+forall (Ps : hfstmt -> Prop) (Pss : hfstmt_seq -> Prop),
+(Ps Sskip) ->
+(forall (v : var) (ft : ftype), Ps (Swire v ft)) ->
+(forall (v : var) (r : hfreg),  Ps (Sreg v r)) ->
+(forall (v : var) (m : hfmem),  Ps (Smem v m)) ->
+(forall (v1 v2 : var),          Ps (Sinst v1 v2)) ->
+(forall (v : var) (e : hfexpr), Ps (Snode v e)) ->
+(forall (r : href) (e : hfexpr), Ps (Sfcnct r e)) ->
+(forall (f : href),             Ps (Sinvalid f)) ->
+(forall (cond : hfexpr) (sst : hfstmt_seq), Pss sst -> forall (ssf : hfstmt_seq), Pss ssf -> Ps (Swhen cond sst ssf)) ->
+(Pss Qnil) ->
+(forall (s : hfstmt), Ps s -> forall (ss : hfstmt_seq), Pss ss -> Pss (Qrcons ss s)) ->
+(forall s : hfstmt, Ps s) /\ (forall ss : hfstmt_seq, Pss ss).
+Proof.
+  intros. split.
+  apply Qrcons_ind' with Pss; try done.
+  apply Qrcons_seq_ind' with Ps; try done.
+Qed.
+
+   Lemma Qeqseq_cons : forall (s : hfstmt) (ss1 ss2 : hfstmt_seq), (Qcons s ss1 == Qcons s ss2) = (ss1 == ss2).
+   Proof.
+   intros.
+   destruct (ss1 == ss2) eqn: H ; move /eqP : H => H ;
+         first by rewrite -H eq_refl //.
+   apply negbTE.
+   apply rwP with (P := ~ (Qcons s ss1 == Qcons s ss2)) ; first by apply negP.
+   contradict H.
+   move /eqP : H => H ; injection H ; done.
+   Qed.
+
+   Lemma Qeqseqr_cat : forall (ss1 ss2 ss3 : hfstmt_seq), (Qcat ss1 ss2 == Qcat ss1 ss3) = (ss2 == ss3).
+   Proof.
+   induction ss1.
+   * simpl Qcat ; reflexivity.
+   * simpl Qcat ; intros.
+     rewrite Qeqseq_cons IHss1 //.
+   Qed.
 
   (* Fixpoint Qfoldl {R : Type} (f : R -> hfstmt -> R) (s : hfstmt_seq) (default : R) :=
    match s with Qnil => default
@@ -156,6 +719,34 @@ Section HiFirrtl.
   | Finput : var -> ftype -> hfport
   | Foutput : var -> ftype -> hfport
   .
+
+  Lemma hfport_eq_dec : forall {x y : hfport}, {x = y} + {x <> y}.
+  Proof.  decide equality ; try apply ftype_eq_dec.
+  1,2: destruct (s == s0) eqn: Hs.
+  2,4: move /eqP : Hs => Hs ; right ; exact Hs.
+  1,2: move /eqP : Hs => Hs ; left ; exact Hs.
+  Qed.
+  Definition hfport_eqn (x y : hfport) : bool :=
+  match x, y with
+  | Finput vx fx, Finput vy fy
+  | Foutput vx fx, Foutput vy fy => (vx == vy) && (fx == fy)
+  | _, _ => false
+  end.
+  Lemma hfport_eqP : Equality.axiom hfport_eqn.
+  Proof.
+  rewrite /Equality.axiom /hfport_eqn.
+  intros.
+  destruct x, y ; try (apply ReflectF ; discriminate).
+  1,2: destruct (s == s0) eqn: Hs.
+  2,4: move /eqP : Hs => Hs ; apply ReflectF ; injection ; done.
+  1,2: move /eqP : Hs => Hs ; rewrite -Hs andTb ; clear Hs s0 ;
+       destruct (f == f0) eqn: Hf.
+  2,4: move /eqP : Hf => Hf ; apply ReflectF ; injection ; done.
+  1,2: move /eqP : Hf => Hf ; rewrite -Hf ; clear Hf f0 ;
+       apply ReflectT ; reflexivity.
+  Qed.
+  Canonical hfport_eqMixin := EqMixin hfport_eqP.
+  Canonical hfport_eqType := Eval hnf in EqType hfport hfport_eqMixin.
 
   Inductive hfmodule : Type :=
   | FInmod : var -> seq hfport -> hfstmt_seq -> hfmodule
